Math/Algebra/C2_Groups/C2_2_morphism_theorems/definitions.lean
@@ -1,0 +1,17 @@
+import Math.Algebra.C2_Groups.C2_1_Basics.theorems
+
+-- definition of the homomorphism in the homomorphism-theorem
+def quotient_homomorphism (G : Type u) (H : Type v) [MyGroup G] [MyGroup H]
+(φ : GroupHomomorphism G H) :
+GroupHomomorphism (left_coset' G (ker_to_normal_subgroup φ)) H := {
+  f := λ x => by {
+    obtain ⟨g, _, _⟩ := x
+    exact φ.f g
+  }
+  mul := by {
+    intros a b
+    simp
+    rw [GroupHomomorphism.f]
+    apply φ.mul
+  }
+}
