Math/Algebra/C2_Groups/C2_2_morphism_theorems/theorems.lean
@@ -1,0 +1,5 @@
+import Math.Algebra.C2_Groups.C2_1_Basics.theorems
+
+-- Theorem 2.2.1 (Homomorphism theorem)
+def quotient_homomorphism (G : Type u) (H : Type v) [MyGroup G] [MyGroup H]
+(φ : GroupHomomorphism G H) : GroupHomomorphism (left_coset' G (ker φ)) H
